compiler/backend/languages/thunk_cexpScript.sml
@@ -43,7 +43,7 @@ Definition cns_arities_def:
   cns_arities (Var v :cexp) = {} ∧
   cns_arities (Prim op es) = (
     (case op of
-     | Cons cn => if explode cn ∈ monad_cns then {{explode cn, LENGTH es}} else {}
+     | Cons cn => if explode cn ∈ monad_cns then {} else {{explode cn, LENGTH es}}
      | _ => {}) ∪
     BIGUNION (set (MAP cns_arities es))) ∧
   cns_arities (App e1 es) = cns_arities e1 ∪ BIGUNION (set (MAP cns_arities es)) ∧
